Curve25519Dalek/Specs/Montgomery/MontgomeryPoint/MulClamped.lean
@@ -46,17 +46,17 @@ natural language specs:
 @[progress]
 theorem mul_clamped_spec (P : MontgomeryPoint) (bytes : Array U8 32#usize) :
     mul_clamped P bytes ⦃ res =>
-    (∃ clamped_scalar,
-    h ∣ U8x32_as_Nat clamped_scalar ∧
-    U8x32_as_Nat clamped_scalar < 2 ^ 255 ∧
-    2 ^ 254 ≤ U8x32_as_Nat clamped_scalar ∧
-    let m:= (U8x32_as_Nat clamped_scalar)
-    MontgomeryPoint.mkPoint res = m • (MontgomeryPoint.mkPoint P)) ⦄ := by
-      unfold mul_clamped
-      progress*
-      have := Nat.mod_eq_of_lt  a_post_2
-      rw[this] at res_post
-      exact ⟨a, a_post_1, a_post_2, a_post_3, res_post⟩
+      (∃ clamped_scalar,
+      h ∣ U8x32_as_Nat clamped_scalar ∧
+      U8x32_as_Nat clamped_scalar < 2 ^ 255 ∧
+      2 ^ 254 ≤ U8x32_as_Nat clamped_scalar ∧
+      let m:= (U8x32_as_Nat clamped_scalar)
+      MontgomeryPoint.mkPoint res = m • (MontgomeryPoint.mkPoint P)) ⦄ := by
+  unfold mul_clamped
+  progress*
+  have := Nat.mod_eq_of_lt  a_post2
+  rw[this] at res_post
+  exact ⟨a, a_post1, a_post2, a_post3, res_post⟩
 
 
 end curve25519_dalek.montgomery.MontgomeryPoint
